proofs/itrees/hoare_logic.v
@@ -1,0 +1,668 @@
+From Coq Require Import
+     Arith.PeanoNat
+     Lists.List
+     Strings.String
+     Morphisms
+     Setoid
+     RelationClasses
+     EquivDec
+     Equality
+     Program.Tactics.
+
+From ExtLib Require Import
+     Data.String
+     Structures.Monad
+     Structures.Traversable
+     Data.List
+     Core.RelDec
+     Structures.Maps
+     Data.Map.FMapAList.
+
+From ITree Require Import
+     ITree
+     ITreeFacts
+     Monad
+     Basics.HeterogeneousRelations
+     Events.Map
+     Events.State
+     Events.StateFacts
+     Events.Reader
+     Events.Exception
+     Events.FailFacts.
+
+Require Import Paco.paco.
+Require Import Psatz.
+Require Import ProofIrrelevance.
+Require Import FunctionalExtensionality.
+
+From mathcomp Require Import ssreflect ssrfun ssrbool ssrnat seq eqtype fintype.
+
+From ITree Require Import
+(*     Basics.Tacs *)
+     Basics.Category
+     Basics.Basics
+     Basics.Function
+     Core.ITreeDefinition
+     Core.KTree
+     Eq.Eqit
+     Eq.UpToTaus
+     Eq.Paco2
+     Indexed.Sum
+     Indexed.Function
+     Indexed.Relation
+     Interp.Handler
+     Interp.Interp
+     Interp.InterpFacts
+     Interp.Recursion.
+
+From ITree Require Import Rutt RuttFacts.
+
+Import Monads.
+Import MonadNotation.
+Local Open Scope monad_scope.
+
+Set Implicit Arguments.
+Unset Strict Implicit.
+Unset Printing Implicit Defensive.
+
+
+Require Import expr psem_defs psem oseq compiler_util xrutt_aux.
+Require Import it_gen_lib it_jasmin_lib it_sems_core core_logics.
+
+(* Definition of a relational logic over program *)
+
+Section Section.
+
+Context
+  {syscall_state : Type}
+  {ep : EstateParams syscall_state}
+  {spp : SemPexprParams}
+  {asm_op: Type}
+  {sip : SemInstrParams asm_op syscall_state}
+  {pT : progT}
+  {wsw : WithSubWord}
+  {scP : semCallParams}
+  {dc : DirectCall}.
+
+Class invEvent (E : Type -> Type) :=
+  { PreInv  :: prepred E
+  ; PostInv :: postpred E }.
+
+Definition Pred (T : Type) := T -> Prop.
+Definition Pred_io (T1 T2 : Type) := T1 -> T2 -> Prop.
+
+Definition PreF := funname -> Pred fstate.
+Definition PostF := funname -> Pred_io fstate fstate.
+
+Definition Pred_e  := Pred pexpr.
+Definition Pred_v  := Pred value.
+Definition Pred_vs := Pred values.
+Definition Pred_c  := Pred estate.
+
+Section TR_MutualRec.
+
+Class hoare_spec :=
+  { preF  : PreF
+  ; postF : PostF }.
+
+Context (spec : hoare_spec) {E: Type -> Type} {wE: with_Error E}.
+
+Definition PreD T (d : recCall T) : Prop :=
+  match d with
+  | RecCall fn fs => preF fn fs
+  end.
+
+Definition PostD T (d : recCall T) (t: T) : Prop :=
+  match d in recCall T_ return T_ -> Prop with
+  | RecCall fn fs => postF fn fs
+  end t.
+
+Definition invEvent_recCall {IE : invEvent E} : invEvent (recCall +' E) :=
+  {| PreInv := sum_prepred (@PreD) PreInv; PostInv := sum_postpred (@PostD) PostInv|}.
+
+End TR_MutualRec.
+
+Section RHOARE.
+
+Context {Err : Set}.
+
+Definition fresult T1 T2 := T1 -> result Err T2.
+
+(* P : precondition
+   Q : postcondition
+   QE : postcondition for error *)
+
+Definition rhoare_io {I O}
+   (P : Pred I) (F : fresult I O) (Q : Pred_io I O) (QE : I -> Pred Err) :=
+  forall i, P i ->
+    match F i with
+    | Ok o => Q i o
+    | Error e => QE i e
+    end.
+
+Definition rhoare {I O} (P : Pred I) (F : fresult I O) (Q : Pred O) (QE : I -> Pred Err) :=
+  rhoare_io P F (fun _ => Q) QE.
+
+Lemma rhoare_ioP {I O} (P : Pred I) (F : fresult I O) (Q : Pred_io I O) (QE : I -> Pred Err) :
+  rhoare_io P F Q QE <-> (forall i0, rhoare (fun i => i = i0 /\ P i) F (Q i0) QE).
+Proof.
+  split.
+  + by move=> h i0 i [? hP]; have := h _ hP; subst i0.
+  by move=> h i hP; apply (h i i).
+Qed.
+
+Lemma rhoare_io_weaken {I O} (F : fresult I O)
+  (P P' : Pred I) (Q Q': Pred_io I O) (QE QE' : I -> Pred Err) :
+  (forall i, P' i -> P i) ->
+  (forall i o, P' i -> Q i o -> Q' i o) ->
+  (forall i e, P' i -> QE i e -> QE' i e) ->
+  rhoare_io P F Q QE ->
+  rhoare_io P' F Q' QE'.
+Proof.
+  move=> hP'P hQQ' hEE' hhoare i hP'.
+  case: (F i) (hhoare i (hP'P i hP')).
+  + by move=> o; apply hQQ'.
+  by move=> e; apply hEE'.
+Qed.
+
+Lemma rhoare_weaken {I O} (F : fresult I O) (P P' : Pred I) (Q Q': Pred O) (QE QE' : I -> Pred Err) :
+  (forall i, P' i -> P i) ->
+  (forall o, Q o -> Q' o) ->
+  (forall i e, P' i -> QE i e -> QE' i e) ->
+  rhoare P F Q QE ->
+  rhoare P' F Q' QE'.
+Proof.
+  move=> hP'P hQQ'; apply rhoare_io_weaken => //.
+  move=> > ?; apply hQQ'.
+Qed.
+
+Lemma rhoare_ok {T} (Q : Pred T) (QE : T -> Pred Err) :
+  rhoare Q (fun t => ok t) Q QE.
+Proof. done. Qed.
+
+Lemma rhoare_Error {T} (P Q : Pred T) (QE : T -> Pred Err) e:
+  (forall t, P t -> QE t e) <->
+  rhoare P (fun t => Error e) Q QE.
+Proof. done. Qed.
+
+Lemma rhoare_bind {I T O} (F1 : fresult I T) (F2 : fresult T O)
+  (P : Pred I) (R : Pred T) (Q : Pred O) (QE : I -> Pred Err) (QET : T -> Pred Err) :
+  (forall i t e , P i -> R t -> QET t e -> QE i e) ->
+  rhoare P F1 R QE ->
+  rhoare R F2 Q QET ->
+  rhoare P (fun i => Let r := F1 i in F2 r) Q QE.
+Proof.
+  move=> hQE hF1 hF2 i hP.
+  case: (F1 i) (hF1 i hP) => //=.
+  move=> t hR; case: (F2 t) (hF2 t hR) => //=.
+  by move=> e; apply hQE.
+Qed.
+
+Lemma rhoare_read {S T O} (F1 : fresult S T) (F2 : T -> fresult S O)
+  (P : Pred S) (R : Pred T) (Q : Pred O) (QE : S -> Pred Err) :
+  rhoare P F1 R QE ->
+  (forall t, R t -> rhoare P (F2 t) Q QE) ->
+  rhoare P (fun s => Let r := F1 s in F2 r s) Q QE.
+Proof.
+  move=> hF1 hF2 s hP.
+  case: (F1 s) (hF1 s hP) => //=.
+  move=> t hR; case: (F2 t s) (hF2 t hR s hP) => //=.
+Qed.
+
+Lemma rhoare_bind_eval {S I T O} (F1 : fresult I T) (F2 : T -> fresult S O)
+  (P : Pred S) (R : Pred T) (Q : Pred O) (QE : S -> Pred Err) i :
+  (forall s, P s -> rhoare (fun i' => i' = i) F1 R (fun _ => QE s)) ->
+  (forall t, R t -> rhoare P (F2 t) Q QE) ->
+  rhoare P (fun s => Let r := F1 i in F2 r s) Q QE.
+Proof.
+  move=> hF1 hF2 s hP.
+  case: (F1 i) (hF1 s hP i erefl) => //=.
+  move=> t hR; case: (F2 t s) (hF2 t hR s hP) => //=.
+Qed.
+
+Lemma rhoare_eval {S I O} (F : fresult I O)
+  (P : Pred S) (Q : Pred O) (QE : S -> Pred Err) i :
+  (forall s, P s -> rhoare (fun i' => i' = i) F Q (fun _ => QE s)) ->
+  rhoare P (fun s => F i) Q QE.
+Proof. by move=> hF s hP; case: (F i) (hF s hP i erefl). Qed.
+
+Lemma rhoare_write {S O} (F1 : fresult S S) (F2 : fresult S O)
+  (P R : Pred S) (Q : Pred O) (QE : S -> Pred Err) :
+  rhoare_io P F1 (fun s s' => R s' /\ forall e, QE s' e -> QE s e) QE ->
+  rhoare R F2 Q QE ->
+  rhoare P (fun s => Let s := F1 s in F2 s) Q QE.
+Proof.
+  move=> hF1 hF2 s hP.
+  case: (F1 s) (hF1 s hP) => //=.
+  by move=> s' [hR hQE]; case: (F2 s') (hF2 s' hR).
+Qed.
+
+Lemma rhoare_id {I O} (F : fresult I O) i0 (P : Pred I) (QE : I -> Pred Err):
+  rhoare (fun i => i = i0 /\ P i) F (fun=> True) QE ->
+  rhoare (fun i => i = i0 /\ P i) F (fun o => F i0 = ok o) QE.
+Proof.
+  by move=> h i hP; have := h i hP; case: hP => ? _; subst i0; case: (F i).
+Qed.
+
+End RHOARE.
+
+Section KHOARE.
+
+Context {E: Type -> Type} {wE: with_Error E} {rE : invEvent E}.
+
+Definition khoare_io {I O}
+   (P : Pred I) (F : ktree E I O) (Q : Pred_io I O) :=
+  forall i, P i -> lutt PreInv PostInv (Q i) (F i).
+
+Definition khoare {I O} (P : Pred I) (F : ktree E I O) (Q : Pred O) :=
+  khoare_io P F (fun i => Q).
+
+(* Remark: in pratice khoare_io and khoare are equivalent *)
+Lemma khoare_ioP {I O} (P : Pred I) (F : ktree E I O) (Q : Pred_io I O) :
+  khoare_io P F Q <-> (forall i0, P i0 -> khoare (fun i => i = i0 /\ P i) F (Q i0)).
+Proof.
+  split.
+  + by move=> h i0 _ i [? hP]; have := h _ hP; subst i0.
+  by move=> h i hP; apply (h i hP i).
+Qed.
+
+Lemma khoare_io_weaken {I O} (P P' : Pred I) (Q Q': Pred_io I O) F :
+  (forall i, P' i -> P i) ->
+  (forall i o, P' i -> Q i o -> Q' i o) ->
+  khoare_io P F Q ->
+  khoare_io P' F Q'.
+Proof.
+  move=> hP'P hQQ' heqv i hP'.
+  apply lutt_weaken with PreInv PostInv (Q i) => //.
+  + by move=> >; apply hQQ'.
+  by apply/heqv/hP'P.
+Qed.
+
+Lemma khoare_weaken {I O} (P P' : Pred I) (Q Q': Pred O) F :
+  (forall i, P' i -> P i) ->
+  (forall o, Q o -> Q' o) ->
+  khoare P F Q ->
+  khoare P' F Q'.
+Proof. move=> hP hQ; apply khoare_io_weaken => // > _; apply hQ. Qed.
+
+Lemma khoare_io_ret {I O} (P: Pred I) (f : I -> O) (Q : Pred_io I O) :
+  (forall i, P i -> Q i (f i)) ->
+  khoare_io P (fun i => ret (f i)) Q.
+Proof. by move=> hPQ i hP; rewrite -lutt_Ret; apply hPQ. Qed.
+
+Lemma khoare_ret {I O} (P : Pred I) (f : I -> O) (Q : Pred O) :
+  (forall i, P i -> Q (f i)) ->
+  khoare P (fun i => ret (f i)) Q.
+Proof. by apply khoare_io_ret. Qed.
+
+Lemma khoare_io_bind {I T O}
+  (R : Pred_io I T)
+  (P : Pred I)
+  (Q : Pred_io I O) F F' :
+  khoare_io P F R ->
+  (forall i, P i -> khoare (R i) F' (Q i)) ->
+  khoare_io P (fun i => t <- F i;; F' t) Q.
+Proof.
+  move=> h h' i hP.
+  apply lutt_bind with (R i); first by apply h.
+  by move=> t hR; apply h'.
+Qed.
+
+Lemma khoare_bind {I T O}
+  (R : Pred T)
+  (P : Pred I)
+  (Q : Pred O) F F' :
+  khoare P F R ->
+  khoare R F' Q ->
+  khoare P (fun i => t <- F i;; F' t) Q.
+Proof. by move=> h h'; apply khoare_io_bind with (R := fun t => R). Qed.
+
+Definition Qerr (s : estate) e := PreInv (subevent void (Throw (mk_error_data s e))).
+
+Lemma khoare_io_iresult (T : Type) F (P : Pred_c) (Q: Pred_io estate T) :
+  rhoare_io P F Q Qerr ->
+  khoare_io P (fun s => iresult s (F s)) Q.
+Proof.
+  move=> hr s hP; have := hr s hP.
+  case: (F s) => [v | e] hQ.
+  + by apply lutt_Ret.
+  by apply lutt_Vis.
+Qed.
+
+Lemma khoare_iresult (T : Type) F (P : Pred_c) (Q: Pred T) :
+  rhoare P F Q Qerr ->
+  khoare P (fun s => iresult s (F s)) Q.
+Proof. apply khoare_io_iresult. Qed.
+
+Lemma khoare_read {S T O} (F1 : ktree E S T) (F2 : T -> ktree E S O)
+  (P : Pred S) (R : Pred T) (Q : Pred O) :
+  khoare P F1 R ->
+  (forall t, R t -> khoare P (F2 t) Q) ->
+  khoare P (fun s => r <- F1 s ;; F2 r s) Q.
+Proof.
+  move=> hF1 hF2 s hP.
+  eapply lutt_bind; eauto.
+  by move=> t hR; apply hF2.
+Qed.
+
+Lemma khoare_eval {S I T O} (F1 : ktree E I T) (F2 : T -> ktree E S O)
+  (P : Pred S) (R : Pred T) (Q : Pred O) i :
+  (forall s, P s -> khoare (fun i' => i' = i) F1 R) ->
+  (forall t, R t -> khoare P (F2 t) Q) ->
+  khoare P (fun s => r <- F1 i ;; F2 r s) Q.
+Proof.
+  move=> hF1 hF2 s hP.
+  eapply lutt_bind.
+  + by apply (hF1 _ hP i erefl).
+  by move=> t hR; apply hF2.
+Qed.
+
+Lemma khoare_eq_pred {I O} (F : ktree E I O) (P : Pred I) (Q : Pred O) :
+  (forall i0, khoare (fun i => i = i0 /\ P i) F Q) ->
+  khoare P F Q.
+Proof. by move=> h i0 hP; apply (h i0 i0). Qed.
+
+Lemma khoare_iter (IT T : Type) (I : Pred IT) (Q : Pred T) (body : ktree E IT (IT + T)) :
+  khoare I body (sum_pred I Q) ->
+  khoare I (ITree.iter body) Q.
+Proof. move=> hbody i hI; apply: lutt_iter hI => {}i; apply hbody. Qed.
+
+End KHOARE.
+
+Section HOARE_CORE.
+
+Context {E : Type -> Type} {wE: with_Error E} {inv : invEvent E}.
+Context {sem_F : sem_Fun E} (p : prog) (ev: extra_val_t).
+
+Definition hoare_f (P : PreF) (fn : funname) (Q: PostF) :=
+  khoare_io (P fn) (sem_fun p ev fn) (Q fn).
+
+Definition hoare_f_body (P : PreF) (fn : funname) (Q:PostF) :=
+  khoare_io (P fn) (isem_fun_body p ev fn) (Q fn).
+
+Definition hoare_io (P : Pred_c) (c : cmd) (Q : Pred_io estate estate) :=
+  khoare_io P (isem_cmd_ p ev c) Q.
+
+Definition hoare (P : Pred_c) (c : cmd) (Q : Pred_c) :=
+  khoare P (isem_cmd_ p ev c) Q.
+
+(* Since hoare_io and hoare are equivalent we will only focus on hoare *)
+Lemma hoare_ioP P c Q :
+  hoare_io P c Q <-> (forall s0, P s0 -> hoare (fun s => s = s0 /\ P s) c (Q s0)).
+Proof. apply khoare_ioP. Qed.
+
+(* FIXME allow to weaken the invPred *)
+Lemma hoare_weaken P1 P2 Q1 Q2 c :
+  (forall s, P1 s -> P2 s) ->
+  (forall s, Q2 s -> Q1 s) ->
+  hoare P2 c Q2 ->
+  hoare P1 c Q1.
+Proof. apply khoare_weaken. Qed.
+
+Lemma hoare_cat (R P Q : Pred_c) (c c' : cmd) :
+  hoare P c R ->
+  hoare R c' Q ->
+  hoare P (c ++ c') Q.
+Proof.
+  move=> h h' s hP ; rewrite isem_cmd_cat.
+  apply lutt_bind with R => //.
+  by apply h.
+Qed.
+
+Lemma hoare_nil Q : hoare Q [::] Q.
+Proof. move=> hQ; apply lutt_Ret. Qed.
+
+Lemma hoare_cons (R P Q : Pred_c) (i : instr) (c : cmd) :
+  hoare P [::i] R ->
+  hoare R c Q ->
+  hoare P (i :: c) Q.
+Proof. rewrite -(cat1s i c); apply hoare_cat. Qed.
+
+Lemma hoare_assgn (Rv Rtr: Pred_v) (P Q : Pred_c) ii x tg ty e :
+  rhoare P (fun s => sem_pexpr true (p_globs p) s e) Rv Qerr ->
+  (forall s, P s -> rhoare Rv (truncate_val ty) Rtr (fun _ => Qerr s)) ->
+  (forall v, Rtr v -> rhoare P (write_lval true (p_globs p) x v) Q Qerr) ->
+  hoare P [:: MkI ii (Cassgn x tg ty e)] Q.
+Proof.
+  move=> he htr hwr; rewrite /hoare /isem_cmd_ /=.
+  apply khoare_bind with Q; last by apply khoare_ret.
+  apply khoare_iresult; rewrite /sem_assgn.
+  apply: (rhoare_read he) => v hv.
+  apply rhoare_bind_eval with Rtr.
+  + by move=> s /htr; apply rhoare_weaken => // > ->.
+  apply hwr.
+Qed.
+
+Lemma hoare_opn (Rve Rvo : Pred_vs) P Q ii xs tag o es :
+  rhoare P (fun s => sem_pexprs true (p_globs p) s es) Rve Qerr ->
+  (forall s, P s -> rhoare Rve (exec_sopn o) Rvo (fun _ => Qerr s)) ->
+  (forall vs, Rvo vs -> rhoare P (fun s => write_lvals true (p_globs p) s xs vs) Q Qerr) ->
+  hoare P [:: MkI ii (Copn xs tag o es)] Q.
+Proof.
+  move=> he ho hwr; rewrite /hoare /isem_cmd_ /=.
+  apply khoare_bind with Q; last by apply khoare_ret.
+  apply khoare_iresult; rewrite /sem_sopn.
+  eapply rhoare_read.
+  + eapply rhoare_read; first apply he.
+    move=> t ht; eapply rhoare_eval.
+    move=> s /ho; apply rhoare_weaken; last done.
+    + by move=> > ->.
+    by move=> > h; apply h.
+  by apply hwr.
+Qed.
+
+Lemma hoare_syscall Rv Ro P Q ii xs sc es :
+  rhoare P (fun s => sem_pexprs true (p_globs p) s es) Rv Qerr ->
+  (forall s, P s ->
+     rhoare Rv (fun vs => fexec_syscall sc (mk_fstate vs s)) Ro (fun _ => Qerr s)) ->
+  (forall fs, Ro fs ->
+     rhoare P (upd_estate true (p_globs p) xs fs) Q Qerr) ->
+  hoare P [:: MkI ii (Csyscall xs sc es)] Q.
+Proof.
+  move=> he ho hwr; rewrite /hoare /isem_cmd_ /=.
+  apply khoare_bind with Q; last by apply khoare_ret.
+  apply khoare_iresult; rewrite /sem_syscall.
+  apply (rhoare_read he).
+  move=> t ht; eapply rhoare_read; last by apply hwr.
+  move=> s hP; apply (ho s hP _ ht).
+Qed.
+
+Lemma hoare_if_full P Q ii e c c' :
+  rhoare P (sem_cond (p_globs p) e) (fun _ => True) Qerr ->
+  (forall b,
+     hoare (fun s => P s /\ sem_cond (p_globs p) e s = ok b) (if b then c else c') Q) ->
+  hoare P [:: MkI ii (Cif e c c')] Q.
+Proof.
+  move=> he hc; rewrite /hoare /isem_cmd_ /=.
+  apply khoare_bind with Q; last by apply khoare_ret.
+  apply khoare_eq_pred => s0.
+  apply khoare_read with (fun b => sem_cond (p_globs p) e s0 = ok b).
+  + rewrite /isem_cond; apply khoare_iresult.
+    by apply rhoare_id; apply: rhoare_weaken he => // > [].
+  by move=> b hb; apply: khoare_weaken (hc b) => // s [->].
+Qed.
+
+Lemma hoare_if P Q ii e c c' :
+  rhoare P (sem_cond (p_globs p) e) (fun _ => True) Qerr ->
+  (forall b, hoare P (if b then c else c') Q) ->
+  hoare P [:: MkI ii (Cif e c c')] Q.
+Proof.
+  move=> he hc; apply hoare_if_full => //.
+  by move=> b; apply: hoare_weaken (hc b) => // s [].
+Qed.
+
+Lemma hoare_for_full P Pb Pi ii i d lo hi c :
+  rhoare P (sem_bound (p_globs p) lo hi) Pb Qerr ->
+  (forall bounds (j:Z),
+    Pb bounds ->
+    (* FIXME : j \in (wrange d bounds.1 bounds.2) *)
+    List.In j (wrange d bounds.1 bounds.2) ->
+    rhoare P (write_var true i (Vint j)) Pi Qerr) ->
+  hoare Pi c P ->
+  hoare P [:: MkI ii (Cfor i (d, lo, hi) c)] P.
+Proof.
+  move=> hbound hwi hc; rewrite /hoare /isem_cmd_ /=.
+  apply khoare_bind with P; last by apply khoare_ret.
+  apply khoare_read with Pb.
+  + by apply khoare_iresult.
+  move=> bounds {}/hwi; elim (wrange _ _) => /= [ | j js hrec] hwi.
+  + by apply khoare_ret.
+  eapply khoare_bind.
+  + by apply khoare_iresult; apply hwi; left.
+  by apply: (khoare_bind hc); apply hrec => z hz; apply hwi; right.
+Qed.
+
+Lemma hoare_for P Pi ii i d lo hi c :
+  rhoare P (sem_bound (p_globs p) lo hi) (fun _ => True) Qerr ->
+  (forall (j:Z), rhoare P (write_var true i (Vint j)) Pi Qerr) ->
+  hoare Pi c P ->
+  hoare P [:: MkI ii (Cfor i (d, lo, hi) c)] P.
+Proof.
+  move=> hbound hwi.
+  apply: (hoare_for_full ii hbound) => _ j _ _; apply hwi.
+Qed.
+
+Lemma hoare_while_full I I' ii al e c c' :
+  hoare I c I' ->
+  rhoare I' (sem_cond (p_globs p) e) (fun _ => True) Qerr  ->
+  hoare (fun s => I' s /\ sem_cond (p_globs p) e s = ok true) c' I ->
+  hoare I [:: MkI ii (Cwhile al c e c')]
+     (fun s => I' s /\ sem_cond (p_globs p) e s = ok false).
+Proof.
+  move=> hc he hc'; rewrite /hoare /isem_cmd_ /=.
+  set Q := (Q in khoare _ _ Q).
+  apply khoare_bind with Q; last by move=> >; apply: khoare_ret.
+  apply khoare_iter.
+  apply: (khoare_bind hc).
+  apply khoare_eq_pred => s0.
+  apply khoare_read with (fun b => sem_cond (p_globs p) e s0 = ok b).
+  + apply khoare_iresult.
+    by apply rhoare_id; apply: rhoare_weaken he => // > [].
+  move=> [] hb; last first.
+  + by apply khoare_ret => _ [-> ?]; constructor.
+  apply khoare_bind with I.
+  + by apply: khoare_weaken hc' => // _ [-> ?].
+  by apply khoare_ret.
+Qed.
+
+Lemma hoare_while I I' ii al e c c' :
+  hoare I c I' ->
+  rhoare I' (sem_cond (p_globs p) e) (fun _ => True) Qerr  ->
+  hoare I' c' I ->
+  hoare I [:: MkI ii (Cwhile al c e c')] I'.
+Proof.
+  move=> hc hcond hc'.
+  apply hoare_weaken with I (fun s => I' s /\ sem_cond (p_globs p) e s = ok false) => //.
+  + by move=> ? [].
+  apply hoare_while_full => //.
+  by apply: hoare_weaken hc' => // ? [].
+Qed.
+
+Lemma hoare_call (Pf : PreF) (Qf : PostF) Rv P Q ii xs fn es :
+  rhoare P (fun s => sem_pexprs (~~ direct_call) (p_globs p) s es) Rv Qerr ->
+  (forall s vs, P s -> Rv vs -> Pf fn (mk_fstate vs s)) ->
+  hoare_f Pf fn Qf ->
+  (forall fs fr,
+    Pf fn fs -> Qf fn fs fr ->
+    rhoare P (upd_estate (~~ direct_call) (p_globs p) xs fr) Q Qerr) ->
+  hoare P [:: MkI ii (Ccall xs fn es)] Q.
+Proof.
+  move=> hes hPPf hCall hPQf; rewrite /hoare /isem_cmd_ /=.
+  apply khoare_bind with Q; last by apply khoare_ret.
+  apply khoare_read with Rv.
+  + by apply khoare_iresult => >; apply: hes.
+  move=> vs hvs; apply khoare_eq_pred => s0.
+  set (fs := mk_fstate vs s0).
+  apply khoare_read with (Qf fn fs).
+  + by move=> _ [-> hP]; apply/hCall/hPPf.
+  move=> fr hQf; apply khoare_iresult.
+  move=> _ [-> hP]; apply (hPQf fs fr) => //.
+  by apply hPPf.
+Qed.
+
+Definition hoare_fun_body_hyp (Pf : PreF) fn (Qf : PostF) :=
+  forall fs,
+  Pf fn fs ->
+  match get_fundef (p_funcs p) fn with
+  | None => PreInv (subevent void (Throw (ErrType, tt)))
+  | Some fd =>
+    exists (P Q : Pred_c),
+      [/\ rhoare (Pf fn) (initialize_funcall p ev fd) P (fun _ => Qerr (estate0 fs))
+        , hoare P fd.(f_body) Q
+        & rhoare Q (finalize_funcall fd) (Qf fn fs) Qerr]
+  end.
+
+Lemma hoare_fun_body Pf fn Qf :
+  hoare_fun_body_hyp Pf fn Qf ->
+  hoare_f_body Pf fn Qf.
+Proof.
+  move=> hf; rewrite /hoare_f_body /isem_fun_body.
+  apply khoare_ioP => fs hPf; have {}hf := hf _ hPf.
+  apply khoare_read with (fun fd => get_fundef (p_funcs p) fn = Some fd).
+  + rewrite /kget_fundef => _ [-> _].
+    by case: get_fundef hf => /= [fd | ] h; [apply lutt_Ret | apply lutt_Vis].
+  move=> fd hfd; move: hf; rewrite hfd => -[P] [Q] [hinit hbody hfin].
+  apply khoare_bind with P.
+  + move=> _ [-> _]; have := hinit _ hPf.
+    by case: initialize_funcall => [s | e] h; [apply lutt_Ret | apply lutt_Vis].
+  by apply: (khoare_bind hbody); apply khoare_iresult.
+Qed.
+
+End HOARE_CORE.
+
+Section HOARE_FUN.
+
+Context {E : Type -> Type} {wE: with_Error E} {rE : invEvent E}.
+
+Context (p : prog) (ev: extra_val_t) (spec : hoare_spec).
+
+Definition hoare_f_rec Pf fn Qf :=
+  hoare_f (inv := invEvent_recCall spec) p ev Pf fn Qf.
+
+Definition hoare_rec P c Q :=
+  hoare (inv := invEvent_recCall spec) p ev P c Q.
+
+Definition hoare_fun_body_hyp_rec Pf fn Qf :=
+  forall fs,
+  Pf fn fs ->
+  match get_fundef (p_funcs p) fn with
+  | None => PreInv (subevent void (Throw (ErrType, tt)))
+  | Some fd =>
+    exists (P Q : Pred_c),
+      [/\ rhoare (Pf fn) (initialize_funcall p ev fd) P (fun _ => Qerr (estate0 fs))
+        , hoare_rec P fd.(f_body) Q
+        & rhoare Q (finalize_funcall fd) (Qf fn fs) Qerr]
+  end.
+
+Lemma isem_fun_ind :
+  ((forall fn, hoare_f_rec preF fn postF) ->
+   forall fn, hoare_fun_body_hyp_rec preF fn postF) ->
+  forall fn, hoare_f p ev preF fn postF.
+Proof.
+  have hrec : (forall fn, hoare_f_rec preF fn postF).
+  + move=> fn' fs' hpre'; apply lutt_trigger.
+    + by apply sum_prepred_inl.
+    by rewrite /PostInv /= => fr h; dependent destruction h.
+  move=> /(_ hrec) hbody.
+  have {}hbody : forall fn,  hoare_fun_body_hyp (inv := invEvent_recCall spec) p ev preF fn postF.
+  + move=> fn fs hp.
+    have := hbody fn fs hp.
+    case: get_fundef => [fd | ].
+    + move=> [P [Q [h1 h2 h3]]]; exists P, Q; split => //.
+      + apply: rhoare_weaken h1 => //.
+        by rewrite /Qerr /= => *; constructor.
+      apply: rhoare_weaken h3 => //.
+      by rewrite /Qerr /= => *; constructor.
+    by rewrite /Qerr /= => *; constructor.
+  move=> fn fs hpre.
+  apply interp_mrec_lutt with (DPEv := PreD spec) (DPAns := PostD spec).
+  + move=> {hpre fn fs}.
+    move=> ? [fn fs] /= hpre.
+    by apply (hoare_fun_body (hbody fn) hpre).
+  apply (hoare_fun_body (hbody fn) hpre).
+Qed.
+
+End HOARE_FUN.
+
+End Section.
+
